\documentclass[12pt,a4paper]{amsart}
\usepackage{graphicx}
\usepackage[color=purple!40]{todonotes} %% does the to do stuff
\usepackage{enumitem}
\usepackage{fullpage}
\usepackage{bbm}

\theoremstyle{plain}

\newtheorem{thm}{Theorem}
\newtheorem*{thm*}{Theorem}
\theoremstyle{definition}
\newtheorem{defn}{Definition}
\newtheorem*{defn*}{Definition}

\newcommand{\B}{\mathcal{B}}
\newcommand{\Hrho}{\mathcal{H}_\rho}
\newcommand{\1}{\mathbbm{1}}
\newcommand{\Vr}{V_\rho}
\newcommand{\Lr}{L_\rho}

\author{Luke Armitage}
\title{C$^\ast$-Algebras, and the~Gelfand-Naimark~Theorem}

\begin{document}
\maketitle


\section{Preliminaries}
we will assume knowledge on... \\
brief(er than asst 3) history




\section{Basics}

\subsection{Definitions}
\begin{defn}[C*-algebra]
	
\end{defn}

\todo[inline] {define C*algebras, states, representations, the weak* topology}





\section{Representations of C*-algebras}
\todo[inline]{to include all representation theory, including GNS, CGN and GN}


\begin{thm} [Gelfand- Naimark-Segal]
	If $\rho$ is a state on a $C^\ast$-algebra $A$, then there exists a cyclic representation 
	$\pi_\rho$ of $A$ on a Hilbert space ${H}_\rho$, with unit cyclic vector $x_\rho$, such that 
	\[ 
		\rho(a)~=~ \langle \pi_\rho (a) x_\rho, x_\rho \rangle, ~~~~ \forall a \in A.
	\]
\end{thm}
\begin{proof}
	We will construct from $\rho$ the space $\Hrho$,  representation $\pi_\rho$, 
	and vector $x_\rho$, and demonstrate the required properties.
	
	Consider the \emph{left kernel} of $\rho$:
	\[
		L_\rho := \{t \in A | \rho (t ^\ast t) = 0 \}.
	\]	
	For $a,b \in A$, define $\langle a , b \rangle_0 := \rho(b^\ast a)$.
	Then $L_\rho = \{t\in A | \langle t , t \rangle _0 = 0 \} $, and 
	$\langle \cdot, \cdot \rangle_0$ satisfies
	\begin{enumerate}[label=(\roman*)]
	  \item Linearity in 1st argument: for $a,b\in A$, $\alpha, \beta \in \mathbb{C}$:
		\begin{align*}
		   \langle \alpha a + \beta b, c \rangle_0 
		&= \rho (c^\ast(\alpha a + \beta b)   								\\
		&= \rho (\alpha c^\ast a + \beta c^\ast b)  						\\
		&= \alpha \rho (c^\ast a) + \beta \rho (c^\ast b)					\\
		&= \alpha \langle a , c \rangle_0 + \beta \langle b, c \rangle_0.
		\end{align*}
	  \item Conjugate symmetric: for $a,b \in A$:
	  	\begin{align*}
	  	   \langle b,a \rangle _0 
	  	&= \rho (a^\ast b)													\\
	  	&= \rho ((b^\ast a)^\ast)											\\
	  	&= \overline{\rho (b^\ast a)}										\\
	  	&= \overline{\langle a,b \rangle _0 }.
	  	\end{align*}
	  \item Positive semi-definite. \todo{why?}
	  	\begin{align*}
	  	\end{align*}
	\end{enumerate}
	Note that $\langle \cdot, \cdot \rangle$ is not necessarily positive definite on 
	$A$ -- $L_\rho$ is exactly where this fails.
	
	$L_\rho$ is a linear subspace of $A$: Consider 
	\[
		L:= \{t \in A  | \langle t,a \rangle _0 = 0, ~\forall a \in A \}\subseteq L_\rho.
	\]
	
	For $t \in L_\rho$, by Cauchy-Schwarz we have 
	\[ 
		|\langle t,a \rangle_0|^2 \leq \langle t,t \rangle_0 \langle a,a\rangle_0,~~ \forall a \in A;
	\]
	that is,
	\[
		\langle t,a \rangle _0 = 0, ~~~ \forall a \in A,
	\]
	so $t\in L$ and $L_\rho =L$.
	
	Now, for $a,b \in L$, $\alpha \in \mathbb{C}$ and $c \in A$:
	\[
		\langle \alpha a + b, c \rangle _0 = \alpha \langle a,c \rangle _0 + \langle b,c\rangle _0 = 0,
	\]
	so $\alpha a +b \in L$; also, $\langle 0,c\rangle _0 = 0$ so $0 \in L$. 
	Hence, $L ( =L_\rho ) $ is a linear subspace of $A$.
	
	For $s \in A$, $t\in L_\rho$, by the Cauchy Schwarz inequality [ref] we have 
	\begin{align*}
		|\rho (s^\ast t) |^2 
		&= 		|\langle t,s\rangle_0 |^2 										\\
		&\leq 	\langle t,t\rangle_0 \cdot \langle s,s\rangle_0  				\\
		&= 		\rho (t^\ast t) \cdot \rho (s^\ast s)							\\
		&=		0,
	\end{align*}
	so $\rho (s^\ast t) = 0$. Letting $s = a^\ast a t$ for $a \in A$, then
	\begin{align*}
		\rho ((at)^\ast at) 
		&= 		\rho (at^\ast a^\ast at) 										\\
		&= 		\rho ((a^\ast at)^\ast t) 										\\
		&= 		\rho (s^\ast t) 												\\
		&=		0,
	\end{align*}
	so that $at \in L_\rho$, for all $a \in A$ and $t \in L_\rho$; 
	we conclude that $L_\rho$ is a left ideal in $A$.
	$L_\rho$ is \todo{start sentence properly} the preimage in $A$ of $\{0\}$ under the continuous map 
	$t \mapsto \rho (t^\ast t)$, so is closed.
	
	Consider now $V_\rho := A / L_\rho$, with $\langle \cdot,\cdot\rangle$ defined by 
	\[
		\langle a+L_\rho,b+L_\rho \rangle := \langle a,b\rangle_0, ~~~~ 
		\mbox{for}~~a+L_\rho,b+L_\rho \in V_\rho.
	\]
	It follows from properties $i),ii)$ and $iii)$ of $\langle \cdot,\cdot  \rangle _0$ that
	$\langle \cdot,\cdot  \rangle$ is an inner product on $V_\rho$ - with
	\begin{align*}
				\langle a + L^\rho, a + L^\rho \rangle = 0
		&\iff 	\langle a,a\rangle=0										\\
		&\iff 	a \in L_\rho												\\
		&\iff 	a+L_\rho = 0+L_\rho
	\end{align*}
	giving positive definiteness.
	The completion of $V_\rho$ with respect to $\langle \cdot,\cdot  \rangle$ is a Hilbert space -
	this is the Hilbert space $\Hrho$ we're looking for.
	
	Now we fix $a \in A$, and consider the map 
	\[
		\pi_a : V_\rho \to V_\rho; b+L_\rho \mapsto ab+L_\rho.
	\]
	Let $b_1, b_2 \in A$ be such that $b_1+L_\rho = b_2+L_\rho$. Then:
	\begin{align*}
		&\implies	b_1-b_2 \in L_\rho										\\	
		&\implies	a(b_1-b_2) \in L_\rho									\\	
		&\implies	ab_1-ab_2 \in L_\rho									\\	
		&\implies	ab_1 + L_\rho = ab_2+L_\rho								\\	
		&\implies	\pi_a(b_1+L_\rho) = \pi_a(b_2+L_\rho).
	\end{align*}
	Hence $\pi_a$ defines a linear operator on $V_\rho$.
	
	For $b+L_\rho \in V_\rho$:
	\begin{align*}
				\|a\|^2 \cdot \|b+L_\rho\| - \| \pi_a(b+L_\rho) \|
		&=		\|a\|^2 \cdot \|b+L_\rho\| - \| ab+L_\rho \|				\\
		&=		\|a\|^2 \cdot \langle b+L_\rho,b+L_\rho \rangle - 
									\langle ab+L_\rho,ab+L_\rho \rangle		\\
		&=		\|a\|^2 \cdot \rho(b^\ast b) - \rho ((ab)^\ast ab)			\\
		&= 		\rho (\|a\|^2 b^\ast b-b^\ast a^\ast ab)					\\
		&=		\rho (b^\ast (\|a\|^{2} \mathbbm{1} - a ^\ast a)b)			\\
		&\geq 	0.
	\end{align*}
	
	Thus $\pi_a$ is a bounded operator, with $\|\pi_a\| \leq \|a\|$. By continuity, 
	$\pi_a$ extends to a bounded operator on $\Hrho$ -- say $\pi_\rho(a):\Hrho \to \Hrho$ 
	such that \[ \pi_\rho(a)(v) = \pi_a(v) \] for $v\in \Vr$. 
	Then $\pi_\rho(a) \in \B(\Hrho)$ for each $a \in A$, so $\pi_\rho$ defines a map 
	$A \to \B(\Hrho)$ such that $ a \mapsto \pi_\rho(a)$. This will be our representation.
	
	Now, for $a,b \in A$, $c+ L_\rho \in \Vr$ and $\alpha \in \mathbb{C}$:
	\begin{align*}
				\pi_{\alpha a+b}(c+\Lr)
		&=		(\alpha a+b) (c+\Lr)										\\
		&=		(\alpha ac +\Lr) + (bc+\Lr)									\\
		&=		\alpha \pi_a
	\end{align*}
	
	
	
	
	
	
	
\end{proof}




\end{document}